coq/Correctness.v
@@ -1,0 +1,52 @@
+Require Import Koika.CircuitCorrectness Koika.LoweringCorrectness.
+Require Import Koika.Common Koika.Types Koika.Environments Koika.Logs.
+Require Import Koika.Lowering Koika.CircuitGeneration Koika.CircuitOptimization Koika.Interop.
+
+Section Thm.
+  Context {pos_t var_t rule_name_t reg_t ext_fn_t: Type}.
+  Context {eq_dec_var_t: EqDec var_t}.
+
+  Context {R: reg_t -> type}.
+  Context {Sigma: ext_fn_t -> ExternalSignature}.
+  Context {FiniteType_reg_t: FiniteType reg_t}.
+  Context {Show_var_t : Show var_t}.
+  Context {Show_rule_name_t : Show rule_name_t}.
+
+  Context (r: ContextEnv.(env_t) R).
+  Context (sigma: forall f, Sig_denote (Sigma f)).
+
+  Notation CR := (lower_R R).
+  Notation CSigma := (lower_Sigma Sigma).
+
+  Notation cr := (lower_r r).
+  Notation csigma := (lower_sigma sigma).
+
+  Context (lco: (@local_circuit_optimizer
+                   rule_name_t reg_t ext_fn_t
+                   CR CSigma
+                   (rwdata (rule_name_t := rule_name_t) CR CSigma)
+                   (lower_sigma sigma))).
+
+
+  Section Standalone.
+    Context (s: Syntax.scheduler pos_t rule_name_t).
+    Context (rules: rule_name_t -> TypedSyntax.rule pos_t var_t R Sigma).
+    Context (external: rule_name_t -> bool).
+
+    Theorem compiler_correct:
+      let spec_results := commit_update r (TypedSemantics.interp_scheduler r sigma rules s) in
+      let circuits := compile_scheduler lco rules external s in
+      forall reg,
+        interp_circuit cr csigma (ContextEnv.(getenv) circuits reg) =
+        bits_of_value (ContextEnv.(getenv) spec_results reg).
+    Proof.
+      cbv zeta; intros.
+      setoid_rewrite compile_scheduler'_correct.
+      - rewrite scheduler_lowering_correct.
+        unfold lower_r;
+          rewrite SemanticProperties.commit_update_log_map_values, getenv_map;
+          reflexivity.
+      - apply circuit_env_equiv_CReadRegister.
+    Qed.
+  End Standalone.
+End Thm.
